Nits.

SMC-fill.ec
@@ -1,6 +1,8 @@
 (* Secure Message Communication via a One-time Pad, Formalized
    in Ordinary (Non-UC) Real/Ideal Paradigm Style *)
 
+prover [""].  (* no use of smt *)
+
 require import AllCore Distr.
 
 (* minimal axiomatization of bitstrings *)
@@ -9,7 +11,7 @@ op n : int.  (* length of bitstrings *)
 
 axiom ge0_n : 0 <= n.
 
-type bits.  (* type of bitstrings *)
+type bits.  (* type of bit strings of length n *)
 
 op zero : bits.  (* the all zero bitstring *)
 
@@ -27,7 +29,7 @@ axiom xor0_ (x : bits) :
 lemma xor_0 (x : bits) :
   x ^^ zero = x.
 proof.
-
+by rewrite xorC xor0_.
 qed.
 
 axiom xorK (x : bits) :
@@ -36,13 +38,13 @@ axiom xorK (x : bits) :
 lemma xor_double_same_right (x y : bits) :
   x ^^ y ^^ y = x.
 proof.
-
+by rewrite xorA xorK xor_0.
 qed.
 
 lemma xor_double_same_left (x y : bits) :
   y ^^ y ^^ x = x.
 proof.
-
+by rewrite xorK xor0_.
 qed.
 
 (* uniform, full and lossless distribution on bitstrings *)
@@ -56,7 +58,10 @@ axiom dbits1E (x : bits) :
 
 lemma dbits_fu : is_full dbits.
 proof.
-
+move => x.
+rewrite /support dbits1E.
+by rewrite RField.div1r StdOrder.RealOrder.invr_gt0
+           lt_fromint StdOrder.IntOrder.expr_gt0.
 qed.
 
 (* module type of Adversaries *)
@@ -71,7 +76,9 @@ module type ADV = {
 
   proc obs(x : bits) : unit
 
-  (* give Adversary decryption of received message *)
+  (* give Adversary decryption of received message, and ask it for its
+     boolean judgment (the adversary is trying to differentiate the
+     real and ideal games) *)
 
   proc put(x : bits) : bool
 }.
@@ -82,7 +89,11 @@ module GReal (Adv : ADV) = {
   var pad : bits  (* one-time pad *)
 
   (* generate the one-time pad, sharing with both parties; we're
-     assuming Adversary observes nothing when this happens *)
+     assuming Adversary observes nothing when this happens
+
+     of course, it's not realistic that a one-time pad can be
+     generated and secretly shared, but the parties still need to use
+     a one-time pad for secure communication *)
 
   proc gen() : unit = {
     pad <$ dbits;
@@ -114,7 +125,8 @@ module GReal (Adv : ADV) = {
 (* module type of Simulators *)
 
 module type SIM = {
-  (* choose gets no help to simulate encrypted message *)
+  (* choose gets no help to simulate encrypted message; we specify
+     below that choose can't read/write GReal.pad *)
 
   proc choose() : bits
 }.
@@ -134,23 +146,36 @@ module GIdeal(Sim : SIM, Adv : ADV) = {
   }    
 }.
 
-(* Simulator - part of proof, not security specification *)
+(* our goal is to prove the following security theorem, saying the
+   Adversary is completely unable to distinguish the real and ideal
+   games:
 
-module Sim : SIM = {
+lemma Security (Adv <: ADV{GReal}) &m :
+  exists (Sim <: SIM{GReal}),  (* there is a simulator that can't read/write
+                                  GReal.pad *)
+  Pr[GReal(Adv).main() @ &m : res] =
+  Pr[GIdeal(Sim, Adv).main() @ &m : res].
+*)
+
+(* enter section, so Adversary is in scope *)
+
+section.
+
+(* say Adv and GReal don't read/write each other's globals (GIdeal
+   has no globals) *)
+
+declare module Adv : ADV{GReal}.
+
+(* define simulator as a local module, as security theorem won't
+   depend upon it *)
+
+local module Sim : SIM = {
   proc choose() : bits = {
     var x : bits;
     x <$ dbits;
     return x;
   }
 }.
-
-(* enter section, so Adversary is in scope *)
-
-section.
-
-(* say Adv and GReal don't read/write each other's globals *)
-
-declare module Adv : ADV{GReal}.
 
 local lemma GReal_GIdeal :
   equiv[GReal(Adv).main ~ GIdeal(Sim, Adv).main :
@@ -160,6 +185,7 @@ proof.
 qed.
 
 lemma Sec &m :
+  exists (Sim <: SIM{GReal}),
   Pr[GReal(Adv).main() @ &m : res] =
   Pr[GIdeal(Sim, Adv).main() @ &m : res].
 proof.
@@ -171,6 +197,8 @@ end section.
 (* security theorem *)
 
 lemma Security (Adv <: ADV{GReal}) &m :
+  exists (Sim <: SIM{GReal}),  (* there is a simulator that can't read/write
+                                  GReal.pad *)
   Pr[GReal(Adv).main() @ &m : res] =
   Pr[GIdeal(Sim, Adv).main() @ &m : res].
 proof.
